[C$] Refactor and extend some ASTs.
We introduce an explicit AST fixtype for blocks, corresponding to compound
statements in the concrete syntax (grammar). This also adds support for GCC
label declarations in all three situations in which blocks are used: as compound
statements, as statement expressions, and as function bodies. (Label
declarations at the beginning of function bodies seem unnecessary, because
regular labels already have function scope, but GCC accepts them.)

This required a number of adaptation to the syntax tools as well as to the
transformation tools.

books/kestrel/c/syntax/abstract-syntax-symbols.lisp
@@ -388,6 +388,7 @@
     stmt-case
     make-stmt-labeled
     stmt-compound
+    stmt-compound->block
     make-stmt-compound
     stmt-compound->items
     make-stmt-expr
@@ -410,6 +411,13 @@
     block-item-listp
     block-item-list-fix
     block-item-list-count
+
+    block
+    make-block
+    blockp
+    block-count
+    block->labels
+    block->items
 
     fundefp
     fundef
@@ -477,6 +485,7 @@
     irr-decl
     irr-stmt
     irr-block-item
+    irr-block
     irr-fundef
     irr-transunit-ensemble
     irr-code-ensemble
@@ -532,6 +541,7 @@
     stmt-unambp
     block-item-unambp
     block-item-list-unambp
+    block-unambp
     fundef-unambp
     extdecl-unambp
     extdecl-list-unambp
@@ -599,6 +609,7 @@
     stmt-aidentp
     block-item-aidentp
     block-item-list-aidentp
+    block-aidentp
     fundef-aidentp
     extdecl-aidentp
     extdecl-list-aidentp
@@ -635,6 +646,7 @@
     ldm-stmt
     ldm-block-item
     ldm-block-item-list
+    ldm-block
     ldm-param-declon-list
     ldm-fundef
     ldm-type
@@ -689,6 +701,7 @@
     stmt-types
     block-item-types
     block-item-list-types
+    block-types
     fundef-types
 
     valid-ord-info-case
@@ -754,6 +767,7 @@
     stmt-annop
     block-item-annop
     block-item-list-annop
+    block-annop
     fundef-annop
     extdecl-annop
     extdecl-list-annop
