books/kestrel/c/syntax/parser.lisp
@@ -2730,40 +2730,21 @@
        ((token-punctuatorp token "(") ; (
         (b* (;; We read the next token to see if it is an open curly brace,
              ;; but we also need to check that GCC extensions are supported.
-             ((erp token2 & parstate) (read-token parstate))
+             ((erp token2 span2 parstate) (read-token parstate))
              ((when (and (token-punctuatorp token2 "{") ; ( {
                          (parstate->gcc parstate)))
-              (b* (((erp token3 & parstate) (read-token parstate)))
-                (cond
-                 ;; If token3 is a closed curly brace,
-                 ;; we have an empty block.
-                 ((token-punctuatorp token3 "}") ; ( { }
-                  (b* (((erp last-span parstate) ; ( { } )
-                        (read-punctuator ")" parstate))
-                       (prev-expr (expr-stmt nil))
-                       (prev-span (span-join span last-span)))
-                    (parse-postfix-expression-rest prev-expr
-                                                   prev-span
-                                                   parstate)))
-                 ;; If token 3 is not a closed curly brace,
-                 ;; we must have a non-empty block.
-                 (t ; ( { other
-                  (b* ((parstate ; ( {
-                        (if token3 (unread-token parstate) parstate))
-                       (psize (parsize parstate))
-                       ((erp items & parstate) ; ( { items
-                        (parse-block-item-list parstate))
-                       ((unless (mbt (<= (parsize parstate) (1- psize))))
-                        (reterr :impossible))
-                       ((erp & parstate) ; ( { items }
-                        (read-punctuator "}" parstate))
-                       ((erp last-span parstate) ; ( { items } )
-                        (read-punctuator ")" parstate))
-                       (prev-expr (expr-stmt items))
-                       (prev-span (span-join span last-span)))
-                    (parse-postfix-expression-rest prev-expr
-                                                   prev-span
-                                                   parstate))))))
+              (b* ((psize (parsize parstate))
+                   ((erp block & parstate) ; ( { [labels] [items] }
+                    (parse-block span2 parstate))
+                   ((unless (mbt (<= (parsize parstate) (1- psize))))
+                    (reterr :impossible))
+                   ((erp last-span parstate) ; ( { [labels] [items] } )
+                    (read-punctuator ")" parstate))
+                   (prev-expr (expr-stmt block))
+                   (prev-span (span-join span last-span)))
+                (parse-postfix-expression-rest prev-expr
+                                               prev-span
+                                               parstate)))
              ;; If we do not have an open curly brace,
              ;; or if GCC extensions are not supported,
              ;; we need to parse a possibly ambiguous expression or type name.
@@ -3393,44 +3374,25 @@
        ;; We read another token to handle the case of a statement expression
        ;; separately from the other cases.
        ((token-punctuatorp token "(") ; (
-        (b* (((erp token2 & parstate) (read-token parstate)))
+        (b* (((erp token2 span2 parstate) (read-token parstate)))
           (cond
            ;; If token2 is an open curly brace, and GCC extensions are enabled,
            ;; we must have a statement expression, which we parse,
            ;; and then we parse the rest of the postfix expression if any.
            ((and (token-punctuatorp token2 "{") ; ( {
                  (parstate->gcc parstate))
-            (b* (((erp token3 & parstate) (read-token parstate)))
-              (cond
-               ;; If token3 is a closed curly brace,
-               ;; we must have a statement expression with an empty block,
-               ;; which seems odd but not syntactically wrong.
-               ((token-punctuatorp token3 "}") ; ( { }
-                (b* (((erp last-span parstate) ; ( { } )
-                      (read-punctuator ")" parstate))
-                     (prev-expr (expr-stmt nil))
-                     (prev-span (span-join span last-span)))
-                  (parse-postfix-expression-rest prev-expr prev-span parstate)))
-               ;; If token3 is not a closed curly brace,
-               ;; we must have a statement expression with a non-empty block.
-               ;; We put back token3 and we parse one or more block items.
-               (t ; ( { other
-                (b* ((parstate ; ( {
-                      (if token3 (unread-token parstate) parstate))
-                     (psize (parsize parstate))
-                     ((erp items & parstate) ; ( { items
-                      (parse-block-item-list parstate))
-                     ((unless (mbt (<= (parsize parstate) (1- psize))))
-                      (reterr :impossible))
-                     ((erp & parstate) ; ( { items }
-                      (read-punctuator "}" parstate))
-                     ((erp last-span parstate) ; ( { items } )
-                      (read-punctuator ")" parstate))
-                     (prev-expr (expr-stmt items))
-                     (prev-span (span-join span last-span)))
-                  (parse-postfix-expression-rest prev-expr
-                                                 prev-span
-                                                 parstate))))))
+            (b* ((psize (parsize parstate))
+                 ((erp block & parstate) ; ( { [labels] [items] }
+                  (parse-block span2 parstate))
+                 ((unless (mbt (<= (parsize parstate) (1- psize))))
+                  (reterr :impossible))
+                 ((erp last-span parstate) ; ( { [labels] [items] } )
+                  (read-punctuator ")" parstate))
+                 (prev-expr (expr-stmt block))
+                 (prev-span (span-join span last-span)))
+              (parse-postfix-expression-rest prev-expr
+                                             prev-span
+                                             parstate)))
            ;; If token2 is not an open curly brace,
            ;; or if GCC extensions are not supported,
            ;; the opening parenthesis may start
@@ -3790,39 +3752,24 @@
                  (if strings (span-join span last-span) span)
                  parstate)))
        ((token-punctuatorp token "(") ; (
-        (b* (((erp token2 & parstate) (read-token parstate)))
+        (b* (((erp token2 span2 parstate) (read-token parstate)))
           (cond
            ;; If token2 is an open curly brace, and GCC extensions are enabled,
            ;; we have a statement expression.
            ((and (token-punctuatorp token2 "{") ; ( {
                  (parstate->gcc parstate))
-            (b* (((erp token3 & parstate) (read-token parstate)))
-              (cond
-               ;; If token3 is a closed curly brace,
-               ;; we must have a statement expression with an empty block,
-               ;; which seems odd but not syntactically wrong.
-               ((token-punctuatorp token3 "}") ; ( { }
-                (b* (((erp last-span parstate) ; ( { } )
-                      (read-punctuator ")" parstate)))
-                  (retok (expr-stmt nil)
-                         (span-join span last-span)
-                         parstate)))
-               ;; If token3 is not a closed curly brace,
-               ;; we must have a statement expression with a non-empty block.
-               ;; We put back token3 and we parse one or more block items.
-               (t ; ( { other
-                (b* ((parstate ; ( {
-                      (if token3 (unread-token parstate) parstate))
-                     ((erp items & parstate) ; ( { items
-                      (parse-block-item-list parstate))
-                     ((erp & parstate) ; ( { items }
-                      (read-punctuator "}" parstate))
-                     ((erp last-span parstate) ; ( { items } )
-                      (read-punctuator ")" parstate)))
-                  (retok (expr-stmt items)
-                         (span-join span last-span)
-                         parstate))))))
+            (b* ((psize (parsize parstate))
+                 ((erp block & parstate) ; ( { [labels] [items] }
+                  (parse-block span2 parstate))
+                 ((unless (mbt (<= (parsize parstate) (1- psize))))
+                  (reterr :impossible))
+                 ((erp last-span parstate) ; ( { [labels] [items] } )
+                  (read-punctuator ")" parstate)))
+              (retok (expr-stmt block)
+                     (span-join span last-span)
+                     parstate)))
            ;; If token2 is not an open curly brace,
+           ;; or if GCC extensions are not enabled,
            ;; we must have a parenthesized expression.
            ;; We put back token2 and we parse the expression.
            (t ; ( other
@@ -8906,27 +8853,9 @@
        ;; If token is an open curly brace,
        ;; we must have a compound statement.
        ((token-punctuatorp token "{") ; {
-        (b* (((erp labels & parstate) (parse-*-label-declaration parstate))
-             ((erp token2 span2 parstate) (read-token parstate)))
-          (cond
-           ;; If token2 is a closed curly brace,
-           ;; we have an empty compound statement
-           ;; (with possibly some label declarations).
-           ((token-punctuatorp token2 "}") ; { [labels] }
-            (retok (make-stmt-compound :labels labels :items nil)
-                   (span-join span span2)
-                   parstate))
-           ;; Otherwise, we parse a list of one or more block items.
-           (t ; { [labels] other
-            (b* ((parstate ; { [labels]
-                  (if token2 (unread-token parstate) parstate))
-                 ((erp items & parstate) ; { [labels] blockitems
-                  (parse-block-item-list parstate))
-                 ((erp last-span parstate) ; { [labels] blockitems }
-                  (read-punctuator "}" parstate)))
-              (retok (make-stmt-compound :labels labels :items items)
-                     (span-join span last-span)
-                     parstate))))))
+        (b* (((erp block block-span parstate) ; { [labels] [items] }
+              (parse-block span parstate)))
+          (retok (stmt-compound block) block-span parstate)))
        ;; If token is a semicolon,
        ;; we have an expression statement without expression.
        ((token-punctuatorp token ";") ; ;
@@ -9743,6 +9672,53 @@
 
   ;;;;;;;;;;;;;;;;;;;;;;;;;;;;;;;;;;;;;;;;
 
+  (define parse-block ((open-curly-span spanp) (parstate parstatep))
+    :returns (mv erp
+                 (block blockp)
+                 (span spanp)
+                 (new-parstate parstatep :hyp (parstatep parstate)))
+    :parents (parser parse-exprs/decls/stmts)
+    :short "Parse a block."
+    :long
+    (xdoc::topstring
+     (xdoc::p
+      "This is called after the opening curly brace has already been parsed.
+       The span of that opening curly brace is passed as input,
+       so that this function can return a span for the whole block.")
+     (xdoc::p
+      "First, we parse zero or more label declarations.
+       Then, if there is a closing curly brace,
+       we return a block with no block items
+       (and with any label declarations we parsed).
+       Otherwise, we parse one or more block items,
+       and then the closing curly brace.")
+     (xdoc::p
+      "Note that label declarations are accepted
+       only if @('__label__') is recognized as a keyword
+       (see @(tsee parse-*-label-declaration)),
+       which can only happen when GCC extensions are enabled."))
+    (b* (((reterr) (irr-block) (irr-span) parstate) ; {
+         ((erp labels & parstate) ;; { [labels]
+          (parse-*-label-declaration parstate))
+         ((erp token span parstate) (read-token parstate)))
+      (cond
+       ((token-punctuatorp token "}") ; { [labels] }
+        (retok (make-block :labels labels :items nil)
+               (span-join open-curly-span span)
+               parstate))
+       (t ; { [labels] other
+        (b* ((parstate (if token (unread-token parstate) parstate)) ; { [labels]
+             ((erp items & parstate) ; { [labels] items
+              (parse-block-item-list parstate))
+             ((erp last-span parstate) ; { [labels] items }
+              (read-punctuator "}" parstate)))
+          (retok (make-block :labels labels :items items)
+                 (span-join open-curly-span last-span)
+                 parstate)))))
+    :measure (two-nats-measure (parsize parstate) 20))
+
+  ;;;;;;;;;;;;;;;;;;;;;;;;;;;;;;;;;;;;;;;;
+
   :prepwork ((local (in-theory (disable acl2::member-of-cons)))) ; for speed
 
   ;;;;;;;;;;;;;;;;;;;;;;;;;;;;;;;;;;;;;;;;
@@ -10225,6 +10201,11 @@
           (parsize parstate))
       :rule-classes :linear
       :fn parse-block-item-list)
+    (defret parsize-of-parse-block-uncond
+      (<= (parsize new-parstate)
+          (parsize parstate))
+      :rule-classes :linear
+      :fn parse-block)
     :hints
     (("Goal" :in-theory (enable fix nfix))
      (cond
@@ -10521,7 +10502,10 @@
        '(:expand (parse-block-item parstate)))
       ((acl2::occur-lst '(acl2::flag-is 'parse-block-item-list)
                         clause)
-       '(:expand (parse-block-item-list parstate))))))
+       '(:expand (parse-block-item-list parstate)))
+      ((acl2::occur-lst '(acl2::flag-is 'parse-block)
+                        clause)
+       '(:expand (parse-block open-curly-span parstate))))))
 
   ;;;;;;;;;;;;;;;;;;;;;;;;;;;;;;;;;;;;;;;;
 
@@ -11042,6 +11026,12 @@
                    (1- (parsize parstate))))
       :rule-classes :linear
       :fn parse-block-item-list)
+    (defret parsize-of-parse-block-cond
+      (implies (not erp)
+               (<= (parsize new-parstate)
+                   (1- (parsize parstate))))
+      :rule-classes :linear
+      :fn parse-block)
     :hints
     (("Goal" :in-theory (enable fix nfix))
      (cond
@@ -11254,7 +11244,10 @@
        '(:expand (parse-block-item parstate)))
       ((acl2::occur-lst '(acl2::flag-is 'parse-block-item-list)
                         clause)
-       '(:expand (parse-block-item-list parstate))))))
+       '(:expand (parse-block-item-list parstate)))
+      ((acl2::occur-lst '(acl2::flag-is 'parse-block)
+                        clause)
+       '(:expand (parse-block open-curly-span parstate))))))
 
   ;;;;;;;;;;;;;;;;;;;;;;;;;;;;;;;;;;;;;;;;
 
@@ -11476,53 +11469,21 @@
              ;; where the curly brace starts the body, which we parse.
              ((token-punctuatorp token3 "{")
               ;; [__extension__] declspecs declor [asmspec] [attrspecs] {
-              (b* (((erp token4 span4 parstate) (read-token parstate)))
-                (cond
-                 ;; If token4 is a closed curly brace,
-                 ;; we have an empty compound statement as the body.
-                 ((token-punctuatorp token4 "}")
-                  ;; [__extension__] declspecs declor [asmspec] [attrspecs] { }
-                  (retok (extdecl-fundef
-                          (make-fundef :extension extension
-                                       :spec declspecs
-                                       :declor declor
-                                       :asm? asmspec?
-                                       :attribs attrspecs
-                                       :decls nil
-                                       :body nil
-                                       :info nil))
-                         (span-join span span4)
-                         parstate))
-                 ;; If token4 is anything else,
-                 ;; we put it back (if any) and we parse block items,
-                 ;; followed by a closed curly brace.
-                 (t
-                  ;; [__extension__] declspecs declor [asmspec] [attrspecs]
-                  ;;   { other
-                  (b* ((parstate (if token4 (unread-token parstate) parstate))
-                       ;; [__extension__] declspecs declor [asmspec] [attrspecs]
-                       ;;   {
-                       ((erp items & parstate)
-                        ;; [__extension__] declspecs declor
-                        ;;   [asmspec] [attrspecs]
-                        ;;   { items
-                        (parse-block-item-list parstate))
-                       ((erp last-span parstate)
-                        ;; [__extension__] declspecs declor
-                        ;;   [asmspec] [attrspecs]
-                        ;;   { items }
-                        (read-punctuator "}" parstate)))
-                    (retok (extdecl-fundef
-                            (make-fundef :extension extension
-                                         :spec declspecs
-                                         :declor declor
-                                         :asm? asmspec?
-                                         :attribs attrspecs
-                                         :decls nil
-                                         :body items
-                                         :info nil))
-                           (span-join span last-span)
-                           parstate))))))
+              (b* (((erp block last-span parstate)
+                    ;; [__extension__] declspecs declor [asmspec] [attrspecs]
+                    ;; { [labels] [items] }
+                    (parse-block span parstate)))
+                (retok (extdecl-fundef
+                        (make-fundef :extension extension
+                                     :spec declspecs
+                                     :declor declor
+                                     :asm? asmspec?
+                                     :attribs attrspecs
+                                     :decls nil
+                                     :body block
+                                     :info nil))
+                       (span-join span last-span)
+                       parstate)))
              ;; If token3 is anything else,
              ;; we must have one or more declarations, which we parse.
              ;; Then we parse the compound statement.
@@ -11534,18 +11495,14 @@
                     ;; [__extension__] declspecs declor [asmspec] [attrspecs]
                     ;;   decls
                     (parse-declaration-list parstate))
-                   ((erp & parstate)
+                   ((erp open-curly-span parstate)
                     ;; [__extension__] declspecs declor [asmspec] [attrspecs]
                     ;;   decls {
                     (read-punctuator "{" parstate))
-                   ((erp items & parstate)
+                   ((erp block last-span parstate)
                     ;; [__extension__] declspecs declor [asmspec] [attrspecs]
-                    ;;   decls { items
-                    (parse-block-item-list parstate))
-                   ((erp last-span parstate)
-                    ;; [__extension__] declspecs declor [asmspec] [attrspecs]
-                    ;;   decls { items }
-                    (read-punctuator "}" parstate)))
+                    ;;   decls { [labels] [items] }
+                    (parse-block open-curly-span parstate)))
                 (retok (extdecl-fundef
                         (make-fundef :extension extension
                                      :spec declspecs
@@ -11553,7 +11510,7 @@
                                      :asm? asmspec?
                                      :attribs attrspecs
                                      :decls decls
-                                     :body items
+                                     :body block
                                      :info nil))
                        (span-join span last-span)
                        parstate)))))))))))
