books/kestrel/c/syntax/tests/parser.lisp
@@ -729,7 +729,7 @@
 }"
  :gcc t
  :cond (and (stmt-case ast :compound)
-            (equal (stmt-compound->labels ast)
+            (equal (block->labels (stmt-compound->block ast))
                    (list (list (ident "lab"))))))
 
 (test-parse
@@ -740,7 +740,7 @@
 }"
  :gcc t
  :cond (and (stmt-case ast :compound)
-            (equal (stmt-compound->labels ast)
+            (equal (block->labels (stmt-compound->block ast))
                    (list (list (ident "lab1")
                                (ident "lab2"))))))
 
@@ -753,7 +753,7 @@
 }"
  :gcc t
  :cond (and (stmt-case ast :compound)
-            (equal (stmt-compound->labels ast)
+            (equal (block->labels (stmt-compound->block ast))
                    (list (list (ident "lab1")
                                (ident "lab2"))
                          (list (ident "lab3"))))))
